wip

concurrent/paxos.dfy
@@ -7,12 +7,20 @@ module PaxosSingle {
 		  set u : U | u in m :: u
   }
 
-  datatype Loc = P0 | P1 | P2 | P3 | P4 | P5 | P6 ;
+  function method len(s: set<nat>) : (l: nat)
+    ensures l == |s|
+  {
+    |s|
+  }
 
-  datatype Msg =
-      Proposal(pid: nat, n: int)
-    | Accept(pid: nat, n: int, val: int)
-    | Value(pid: nat, vt: int, v: int);
+  datatype Loc = P0 | P1 | P2 | P3 | P4 | P5 | P6 | P7
+
+  datatype Msg_Acc =
+      Proposal(n: int)
+    | Accept(n: int, val: int)
+
+  datatype Msg_Prop =
+      Value(vt: int, v: int)
 
   method PaxosSingle
     ( Ps : set<nat>
@@ -26,14 +34,16 @@ module PaxosSingle {
     // #########################################################################
     // Proposer local state
     // #########################################################################
-    var X       : map<nat, int> := *; assume (forall p :: p in Ps <==> p in X);
-    var X_T     : map<nat, int> := map p | p in Ps :: (-1);
-    var T       : map<nat, nat> := *; assume (forall p :: p in Ps <==> p in T);
-    var HO      : map<nat, nat> := map p | p in Ps :: 0;
-    var Ready   : map<nat, bool>     := map p | p in Ps :: false;
-    var Decided : map<nat, bool>     := map p | p in Ps :: false;
-    var PC      : map<nat, Loc>      := map p | p in Ps :: P0;
-    var WL_As   : map<nat, set<nat>> := map p | p in Ps :: As;
+    var X        : map<nat, int> := *; assume (forall p :: p in Ps <==> p in X);
+    var X_T      : map<nat, int> := map p | p in Ps :: (-1);
+    var T        : map<nat, nat> := *; assume (forall p :: p in Ps <==> p in T);
+    var HO       : map<nat, nat> := map p | p in Ps :: 0;
+    var Ready    : map<nat, bool>     := map p | p in Ps :: false;
+    var Decided  : map<nat, bool>     := map p | p in Ps :: false;
+    var Prop_PC  : map<nat, Loc>      := map p | p in Ps :: P0;
+    var Prop_WL  : map<nat, set<nat>> := map p | p in Ps :: As;
+    var Prop_WL2 : map<nat, set<nat>> := map p | p in Ps :: As;
+    var Prop_a   : map<nat, nat> := *; assume (forall p :: p in Ps <==> p in Prop_a); assume(forall p,a :: p in Ps && a == Prop_a[p] ==> a in As);
     // #########################################################################
 
     // #########################################################################
@@ -48,15 +58,15 @@ module PaxosSingle {
     // #########################################################################
     // Message soups
     // #########################################################################
-    var Acc_Soup  : map<nat, multiset<Msg>> := map a | a in As :: multiset{};
-    var Prop_Soup : map<nat, multiset<Msg>> := map p | p in Ps :: multiset{};
+    var Acc_Soup  : map<nat, multiset<(nat,Msg_Acc)>>  := map a | a in As :: multiset{};
+    var Prop_Soup : map<nat, multiset<(nat,Msg_Prop)>> := map p | p in Ps :: multiset{};
     // #########################################################################
 
     // #########################################################################
     // Set cardinalities
     // #########################################################################
     var k : map<nat, nat> := map p | p in Ps :: 0;
-    var l : map<nat, nat> := map p | p in Ps :: |As|;
+    var l : map<nat, nat> := map p | p in Ps :: len(As);
     var m : map<nat, nat> := map p | p in Ps :: 0;
     // #########################################################################
 
@@ -67,21 +77,30 @@ module PaxosSingle {
     invariant As == old(As);
     invariant WL_main <= Ps + As;
     invariant
-        ( domain(Vs)      == As
-        && domain(Max)     == As
-        && domain(V)       == As 
-        && domain(V_T)     == As
-        && domain(WL_As)   == Ps
-        && domain(PC)      == Ps
-        && domain(X)       == Ps
-        && domain(X_T)     == Ps
-        && domain(HO)      == Ps
-        && domain(k)       == Ps
-        && domain(l)       == Ps
-        && domain(m)       == Ps
-        && domain(Decided) == Ps
-        && domain(Ready)   == Ps
+        ( domain(Ts)        == As
+        && domain(Max)       == As
+        && domain(V)         == As 
+        && domain(V_T)       == As
+        && domain(Prop_WL)   == Ps
+        && domain(Prop_WL2)  == Ps
+        && domain(Prop_PC)   == Ps
+        && domain(X)         == Ps
+        && domain(X_T)       == Ps
+        && domain(HO)        == Ps
+        && domain(k)         == Ps
+        && domain(l)         == Ps
+        && domain(m)         == Ps
+        && domain(Decided)   == Ps
+        && domain(Ready)     == Ps
+
+        && domain(Acc_Soup)  == As
+        && domain(Prop_Soup) == Ps
+        && domain(Prop_a)    == Ps
         );
+    invariant forall a:nat,pid:nat,msg:Msg_Acc :: a in As && (pid,msg) in Acc_Soup[a] ==> pid in Ps;
+    invariant forall p:nat,pid:nat,msg:Msg_Prop :: p in Ps && (pid,msg) in Prop_Soup[p] ==> pid in As;
+    invariant forall p,a :: p in Ps && a == Prop_a[p] ==> a in As;
+    invariant forall p :: p in Ps ==> Prop_WL[p] <= As && Prop_WL2[p] <= As;
     decreases *
     {
       var processToRun := *; assume processToRun in WL_main;
@@ -90,32 +109,114 @@ module PaxosSingle {
         var a := processToRun;
 
         if Acc_Soup[a] != multiset{} {
-          var msg := *; assume msg in Acc_Soup[a];
+          var pid := *;
+          var msg := *;
+
+          assume (pid,msg) in Acc_Soup[a];
+          Acc_Soup := Acc_Soup[a := Acc_Soup[a] - multiset{(pid,msg)}];
 
           match msg {
-            case Proposal(pid,n) =>
+            case Proposal(n) =>
               if Max[a] < n {
                 Max := Max[a := n];
               }
-          }{
-            case Accept(pid,n,val) =>
+            case Accept(n,val) =>
               if Max[a] <= n {
                 V   := V[a := val];
                 V_T := V_T[a := n];
                 Ts  := Ts[a := Ts[a] + {n}];
               }
-          }{
-            case Value(pid,vt,v) =>
-              {}
+          }
+
+          var vt := V_T[a];
+          var v  := V[a];
+
+          if * {
+            Prop_Soup := Prop_Soup[pid := Prop_Soup[pid] + multiset{(a,Value(vt, v))}];
           }
         }
       }
       else if processToRun in Ps {
         var p := processToRun;
 
+        if Prop_PC[p] == P0 {
+          /* for a in A:
+               <P1>
+               <P2>
+             done
+           */
+          if Prop_WL[p] != {} {
+            var a := *; assume a in Prop_WL[p];
+            assert a in As;
+
+            Prop_a := Prop_a[p := a];
+            Prop_WL := Prop_WL[p := Prop_WL[p] - {a}];
+            Prop_PC := Prop_PC[p := P1];
+          } else {
+            Prop_PC := Prop_PC[p := P3];
+          }
+        } else if Prop_PC[p] == P1 {
+          /* send a (p, Proposal(t))
+           */
+          var a := Prop_a[p];
+          var t := T[p];
+          Acc_Soup := Acc_Soup[a := Acc_Soup[a] + multiset{(p, Proposal(t))}];
+          Prop_PC := Prop_PC[p := P2];
+        } else if Prop_PC[p] == P2 {
+          /* Value(vt,v) <- recvTO(a);
+             if vt > xt {
+               xt <- vt
+               x  <- v
+             }
+             ho <- ho + 1
+           */
+
+          // TODO
+        } else if Prop_PC[p] == P3 {
+          /* if 2 x ho > |A| {
+               ho <- 0
+               ready <- true
+               <P4>
+             }
+           */
+          var ho := HO[p];
+          if ho * 2 > |As| {
+            HO := HO[p := 0];
+            Ready := Ready[p := true];
+            Prop_PC := Prop_PC[p := P4];
+          } else {
+            Prop_PC := Prop_PC[p := P7];
+          }
+        } else if Prop_PC[p] == P4 {
+          /* for a in A:
+               <P5>
+               <P6>
+             done
+           */
+          if Prop_WL2[p] != {} {
+            var a := *; assume a in Prop_WL2[p];
+            assert a in As;
+
+            Prop_a := Prop_a[p := a];
+            Prop_WL2 := Prop_WL2[p := Prop_WL2[p] - {a}];
+            Prop_PC := Prop_PC[p := P5];
+          } else {
+            Prop_PC := Prop_PC[p := P7];
+          }
+        } else if Prop_PC[p] == P4 {
+          // TODO
+        } else if Prop_PC[p] == P5 {
+          // TODO
+        } else if Prop_PC[p] == P6 {
+          // TODO
+        } else if Prop_PC[p] == P7 {
+          var ho := HO[p];
+          if ho * 2 > |As| {
+            Decided := Decided[p := true];
+          }
+          WL_main := WL_main - {p};
+        }
       }
-      
     }
   }
-
 }
